proofmode for heap bijection; proofmode fixes

theories/base_logic/gen_heap_bij.v
@@ -26,11 +26,16 @@ Section gset_bij.
   Qed.
 End gset_bij.
 
+Class gen_heap_bij_preG `{gen_sim_heapG L_t L_s V_t V_s Σ} := GenHeapBijPreG {
+  gen_heap_bij_pre_bijG :> gset_bijG Σ L_t L_s;
+}.
 
 Class gen_heap_bijG `{gen_sim_heapG L_t L_s V_t V_s Σ} := GenHeapBijG {
   gen_heap_bij_bijG :> gset_bijG Σ L_t L_s;
   gen_heap_bij_name : gname;
 }.
+Arguments GenHeapBijG L_t L_s V_t V_s Σ {_ _ _ _ _ _} _.
+Arguments gen_heap_bij_name { L_t L_s V_t V_s Σ _ _ _ _ _ _} : assert.
 
 Section definitions.
   Context `{gen_heap_bijG L_t L_s V_t V_s Σ}.
@@ -118,3 +123,20 @@ Section laws.
   Qed.
 
 End laws.
+
+Lemma gen_heap_bij_init_names `{gen_heap_bij_preG L_t L_s V_t V_s Σ} val_rel :
+  ⊢ |==> ∃ γ : gname,
+    let hG := GenHeapBijG L_t L_s V_t V_s Σ γ in
+    gen_heap_bij_inv val_rel.
+Proof.
+  iMod (gset_bij_own_alloc_empty) as (γ) "Hinv".
+  iExists γ. iModIntro. iExists (∅). iSplitL "Hinv"; first by iApply "Hinv".
+  by iApply big_sepS_empty.
+Qed.
+
+Lemma gen_heap_bij_init `{gen_heap_bij_preG L_t L_s V_t V_s Σ} val_rel :
+  ⊢ |==> ∃ _ : gen_heap_bijG, gen_heap_bij_inv val_rel.
+Proof.
+  iMod (gen_heap_bij_init_names val_rel) as (γ) "Hinit".
+  iModIntro. iExists (GenHeapBijG _ _ _ _ _ γ). iFrame.
+Qed.
