theories/simplang/examples/heap_test.v
@@ -3,11 +3,12 @@ From iris Require Import bi.bi.
 Import bi.
 From iris.proofmode Require Import tactics.
 From simuliris.simulation Require Import slsls lifting.
+From simuliris.simplang Require heap_bij.
 
 (** Some very trivial tests for the heap tactics *)
 
 
-Section fix_bi.
+Module fix_bi.
 Context `{sheapG Σ}.
 Instance : sheapRel Σ := {|
   sheap_stateRel _ _ := ⌜True⌝%I;
@@ -51,3 +52,58 @@ Proof.
   target_free. source_free. eauto.
 Qed.
 End fix_bi.
+
+Module bij_test.
+  Import heap_bij.
+  Context `{sbijG Σ}.
+
+  Definition val_rel (v_t v_s : val) :=
+    (match v_t, v_s with
+    | LitV (LitLoc l_t), LitV (LitLoc l_s) => l_t ↔h l_s
+    | _,_ => ⌜v_t = v_s⌝
+    end)%I.
+  Instance : sheapRel Σ := heap_bij_rel val_rel.
+  Instance val_rel_pers v_t v_s : Persistent (val_rel v_t v_s).
+  Proof. destruct v_t as [[] | | | ], v_s as [[] | | | ]; apply _. Qed.
+
+
+  Lemma test_load l l2 :
+    l ↦t #4 -∗ l2 ↦s #4 -∗
+    ((! #l)%E ⪯{val_rel} ! #l2 {{ val_rel }}).
+  Proof.
+    iIntros "H H1". target_load. source_load. eauto.
+  Qed.
+
+  Lemma test_store l l2 :
+    l ↦t #4 -∗ l2 ↦s #4 -∗
+    ((#l <- #42)%E ⪯{val_rel} #l2 <- #1337 {{ val_rel }}).
+  Proof.
+    iIntros "H H1". target_store. source_store. eauto.
+  Qed.
+
+  Lemma test_insert l l2 :
+    l ↦t #4 -∗ l2 ↦s #4 -∗
+    ((#l <- #42)%E ⪯{val_rel} #l2 <- #42 {{ val_rel }}).
+  Proof.
+    iIntros "H H1".
+    iApply (sim_bij_insert val_rel with "H H1 [# ]"); first done; iIntros "Hb".
+    iApply (sim_bij_store with "Hb []"); last by sim_value_head.
+    done.
+  Qed.
+
+  Lemma test_bij_store (l_t l_s : loc) :
+    l_t ↔h l_s -∗
+    (#l_t <- #42)%E ⪯{val_rel} (#l_s <- #42)%E {{ val_rel }}.
+  Proof. 
+    iIntros "H". sim_store; first done. done.
+  Qed.
+  
+
+  Lemma test_bij_load (l_t l_s : loc) : 
+    l_t ↔h l_s -∗
+    ! #l_t ⪯{val_rel} ! #l_s {{ val_rel }}.
+  Proof. 
+    iIntros "H". sim_load v_t v_s as "Ha". done.
+  Qed.
+
+End bij_test.
